working

MyOCL.thy
@@ -3,17 +3,21 @@ theory MyOCL
 begin
 
 type_synonym var = string
+type_synonym ivar = string
 datatype att = AGE | EMAIL | ID
 datatype as = LECTURERS | STUDENTS
+
+
 
 datatype OCLexp = Int nat 
   | Var var 
   | Eq OCLexp OCLexp
-  | Att var att
-  | As var as
+  | IVar ivar
+  | Att OCLexp att
+  | As OCLexp as
   | Size OCLexp
   | IsEmpty OCLexp
-  | Exists OCLexp var OCLexp
+  | Exists OCLexp OCLexp OCLexp
 
 fun transAtt :: "MyOCL.att \<Rightarrow> MySQL.col" where
 "transAtt MyOCL.AGE = MySQL.AGE" |
@@ -24,16 +28,19 @@ fun transAs :: "MyOCL.as \<Rightarrow> MySQL.col" where
 "transAs MyOCL.STUDENTS = MySQL.STUDENTS" |
 "transAs MyOCL.LECTURERS = MySQL.LECTURERS"
 
-fun evalWithCtx :: "OCLexp \<Rightarrow> Objectmodel \<Rightarrow> var \<Rightarrow> val \<Rightarrow> val" where
+fun evalWithCtx :: "OCLexp \<Rightarrow> Objectmodel \<Rightarrow> OCLexp \<Rightarrow> val \<Rightarrow> val" where
 "evalWithCtx (MyOCL.Int i) om var val = VInt i"
-| "evalWithCtx (MyOCL.Var x) om var val = (if (x = var) then val else (VString x))"
+(* For the time being *)
+| "evalWithCtx (MyOCL.Var x) om (MyOCL.IVar i) val = (VString x)"
+| "evalWithCtx (MyOCL.IVar x) om (MyOCL.IVar i) val = val"
+(* *)
 | "evalWithCtx (MyOCL.Eq e1 e2) om var val = 
 VBool (equalVal (evalWithCtx e1 om var val) (evalWithCtx e2 om var val))" 
-| "evalWithCtx (MyOCL.Att v att) om var val
-= (if (v=var) then (projVal (Col (transAtt att)) val) 
+| "evalWithCtx (MyOCL.Att (Var v) att) om (MyOCL.IVar i) val
+= (if (v=i) then (projVal (Col (transAtt att)) val) 
 else (VList (projValList (Col (transAtt att)) [extPerson v (getPersonList om)])))"
-| "evalWithCtx (MyOCL.As v as) om var val
-= (if (v=var) then (projVal (Col (transAs as)) val) 
+| "evalWithCtx (MyOCL.As (Var v) as) om (MyOCL.IVar i) val
+= (if (v=i) then (projVal (Col (transAs as)) val) 
 else (VList (extCol v (transAs as) (getEnrollmentList om))))"
 | "evalWithCtx (MyOCL.Size exp) om var val
 = VList [VInt (sizeVal (evalWithCtx exp om var val))]"
@@ -42,7 +49,7 @@ else (VList (extCol v (transAs as) (getEnrollmentList om))))"
 | "evalWithCtx (MyOCL.Exists src v body) om var val
 = (evalWithCtx src om var val)"
 
-fun filterWithBody :: "val list \<Rightarrow> var \<Rightarrow> OCLexp \<Rightarrow> Objectmodel \<Rightarrow> val list" where
+fun filterWithBody :: "val list \<Rightarrow> OCLexp \<Rightarrow> OCLexp \<Rightarrow> Objectmodel \<Rightarrow> val list" where
 "filterWithBody Nil var (exp) om = Nil" 
 | "filterWithBody (Cons val vs) var exp om = (if (isTrueVal (evalWithCtx exp om var val)) 
     then (val#(filterWithBody vs var exp om))   
@@ -52,8 +59,8 @@ fun eval :: "OCLexp \<Rightarrow> Objectmodel \<Rightarrow> val list" where
 "eval (MyOCL.Int i) om = [VInt i]"
 | "eval (MyOCL.Var x) om = [VString x]"
 | "eval (MyOCL.Eq e1 e2) om = [VBool (equalValList (eval e1 om) (eval e2 om))]" 
-| "eval (MyOCL.Att v att) om = projValList (Col (transAtt att)) [extPerson v (getPersonList om)]"
-| "eval (MyOCL.As v as) om = extCol v (transAs as) (getEnrollmentList om)"
+(*| "eval (MyOCL.Att (Var v) att) om = projValList (Col (transAtt att)) [extPerson v (getPersonList om)]"*)
+(*| "eval (MyOCL.As (Var v) as) om = extCol v (transAs as) (getEnrollmentList om)"*)
 | "eval (MyOCL.Size exp) om = [VInt (sizeValList (eval exp om))]"
 | "eval (MyOCL.IsEmpty exp) om = [VBool (isEmptyValList (eval exp om))]"
 | "eval (MyOCL.Exists src v body) om = [VBool (\<not> isEmptyValList (filterWithBody (eval src om) v body om))]"
