MyMain.thy
@@ -69,61 +69,52 @@ proof (induct om)
   qed
 qed
 
-lemma lem1: assumes "(0 < sizeValList (filterWithBody
-(extCol self col.LECTURERS list) l
-       (OCLexp.Eq (OCLexp.Var l) (OCLexp.Var caller)) (OM ps list)))"
-  shows "(0 < sizeValList (filterWithBody
-(extCol self col.LECTURERS list) l
-       (OCLexp.Eq (OCLexp.Var l) (OCLexp.Var caller)) (OM ps (a#list))))"
+lemma hide0: "filterWithBody vallist var (OCLexp.Eq e1 e1) om = vallist"
   sorry
 
-lemma lem2: "(0 < sizeValList (filterWithBody
-(extCol self col.LECTURERS list) l
-       (OCLexp.Eq (OCLexp.Var l) (OCLexp.Var caller)) (OM ps list))) =
-  (0 < sizeValList (filterWithBody
-(extCol self col.LECTURERS list) l
-       (OCLexp.Eq (OCLexp.Var l) (OCLexp.Var caller)) (OM ps (a#list))))"
+lemma hide1: "v1 \<noteq> v2 \<Longrightarrow> filterWithBody vallist var (OCLexp.Eq (Var v1) (Var v2)) om = []"
+  sorry
+
+lemma hide3 : "sizeValList (filterWithBody vallist (IVar l) (OCLexp.Eq (IVar l) (OCLexp.Var v2)) (OM ps (a # list)))
+= sizeValList (filterWithBody vallist (IVar l) (OCLexp.Eq (IVar l) (OCLexp.Var v2)) (OM ps list))"
+  sorry
+
+lemma lem1: "eval (MyOCL.As (Var v) as) (OM ps []) = []"
+  sorry
+
+
+lemma [simp]: "isTrueVal (select (VEnrollment a) (exp.Eq (exp.Var self) (Col col.STUDENTS)))
+\<Longrightarrow> 
+(eval (As (OCLexp.Var self) as.LECTURERS) om) 
+= (VEnrollment a)#(eval (As (OCLexp.Var self) as.LECTURERS) (OM ps (a#list)))"
+  sorry
+
+lemma [simp]: "isTrueVal (select (VEnrollment a) (exp.Eq (exp.Var caller) (Col col.LECTURERS)))
+\<Longrightarrow> 
+(filterWithBody ((VEnrollment a)#ls) (IVar l) (OCLexp.Eq (IVar l) (OCLexp.Var caller)) (OM ps (a#list)) 
+= (VEnrollment a)#(filterWithBody ls (IVar l) (OCLexp.Eq (IVar l) (OCLexp.Var caller)) (OM ps (a#list))))"
   sorry
 
 (* self.lecturers→exists(l|l=caller)  = SELECT COUNT *  > 0 FROM Enrollment WHERE self = students
 AND lecturers = caller *)
-lemma assumes differentVars: "self \<noteq> caller \<and> self \<noteq> l \<and> caller \<noteq> l"
-  shows "eval (MyOCL.Exists (MyOCL.As self MyOCL.LECTURERS) l 
-(MyOCL.Eq (MyOCL.Var l) (MyOCL.Var caller))) (OM ps es)
+lemma  "eval (MyOCL.Exists (MyOCL.As (Var self) MyOCL.LECTURERS) (MyOCL.IVar l) 
+(MyOCL.Eq (MyOCL.IVar l) (MyOCL.Var caller))) (OM ps es)
 = exec ((SelectFromWhere (MySQL.GrtThan (CountAll) (MySQL.Int 0)) (Table ENROLLMENT) 
 (WHERE (MySQL.And (MySQL.Eq (MySQL.Var self) (Col col.STUDENTS)) 
 (MySQL.Eq (MySQL.Var caller) (Col col.LECTURERS)))))) (OM ps es)"
+
 proof (induct es)
   case Nil
-  then show ?case by simp
+  then show ?case using lem1 by simp
 next
   case (Cons a list)
-  from this have induction_hypothesis: "(0 < sizeValList (filterWithBody (extCol self col.LECTURERS list) l
-       (OCLexp.Eq (OCLexp.Var l) (OCLexp.Var caller)) (OM ps list))) = 
-        (0 < sizeValList (filterEnrollments
-           (And (exp.Eq (exp.Var self) (Col col.STUDENTS))
-             (exp.Eq (exp.Var caller) (Col col.LECTURERS)))
-           list))" by simp
   then show ?case
-  proof (cases "getAssociationEnd col.STUDENTS a = self")
-    case True
-    assume a_STUDENTS_is_self: "getAssociationEnd col.STUDENTS a = self"
-    show ?thesis
-    proof (cases "getAssociationEnd col.LECTURERS a = caller")
-    case True
-      then show ?thesis using a_STUDENTS_is_self by simp
-    next
-      case False
-      then show ?thesis
-        apply (simp add: a_STUDENTS_is_self)
-        apply (simp add: differentVars)
-        sorry
-    qed
-  next
-    case False
-    then show ?thesis
-      sorry
-  qed
+    apply auto
+
+    
+  
+
+
 qed
 
 end
